\documentclass{article}
\usepackage[utf8]{inputenc}
\usepackage{amsmath}
\usepackage{amsfonts}
\usepackage[numbers]{natbib}
\usepackage{algorithm}
\usepackage{algpseudocode}

\title{QP}
\author{albin.fredriksson }
\date{March 2023}

\begin{document}

\maketitle

\section{Introduction}
Primal:
\begin{align*}
\underset{x}{\text{minimize}} \quad & 0.5 x' H x + c' x\\
\text{subject to} \quad
& A x = b\\
& C x \geq d\\
\end{align*}

Replace $C x \geq d$ with $C x - s = d$ and $s \geq 0$.

Log-barrier:
\begin{align*}
\underset{x}{\text{minimize}} \quad & 0.5 x' H x + c' x - \mu e' \log(s) \\
\text{subject to} \quad
& A x = b\\
& C x - s = d\\
\end{align*}


Lagrangian:
\[
L(x, s, y, z) = 0.5 x' H x + c' x - \mu e' \log(s) + y' (Ax - b) - z' (C x - s - d )
\]
First-order optimality conditions:
\begin{align*}
\nabla_x L(x,s,y,z) &= H x + c + A' y - C' z = 0\\
\nabla_s L(x,s,y,z) &= z - \mu S^{-1}e = 0\\
\nabla_y L(x,s,y,z) &= A x - b = 0\\
-\nabla_z L(x,s,y,z) &= C x - s - d = 0\\
\end{align*}

Rearrangement of the first-order optimality conditions:
\begin{align*}
Hx + A' y - C' z &= -c\\
A x - b &= 0\\
C x - s - d &= 0\\
SZe  &=  \mu e\\
\end{align*}

Step:
\begin{align*}
H(x + \Delta x) + A' (y + \Delta y) - C' (z + \Delta z) &= -c\\
A (x + \Delta x) - b &= 0\\
C (x + \Delta x) - (s + \Delta s) - d &= 0\\
(S + \Delta S) (Z + \Delta Z)e  &=  \mu e\\
\end{align*}
Rearrange with delta on left and drop nonlinear terms in delta:
\begin{align*}
H \Delta x + A' \Delta y - C' \Delta z &= -c - Hx - A' y + C' z \\
A \Delta x &= b - A x\\
C \Delta x - \Delta s &= d - C x + s\\
S \Delta z + Z \Delta s &= \mu e - SZe\\
\end{align*}


Newton step:
\[
\left(
\begin{array}{cccc}
H & A' & C' & 0 \\
A & 0 & 0 & 0\\
C & 0 & 0 & I\\
0 & 0 & -S & -Z
\end{array}
\right)
\left(
\begin{array}{c}
\Delta x\\
\Delta y\\
-\Delta z\\
-\Delta s
\end{array}
\right)
=
-\left(
\begin{array}{c}
Hx + A' y - C' z + c\\
A x - b\\
C x - s - d\\
S Z e - \mu e
\end{array}
\right) =
-\left(
\begin{array}{c}
r_x\\
r_y\\
r_z\\
r_s
\end{array}
\right)
\]
Utilizing that $S \Delta z + Z \Delta s = -r_s$, we get
\[
\Delta s = -Z^{-1} (r_s + S \Delta z)
\]
or, written in another way
\[
-Z^{-1} S \Delta z = \Delta s + Z^{-1} r_s
\]
we can remove $\Delta s$ from the third equation and reduce the system to
\[
\left(
\begin{array}{cccc}
H & A' & C' \\
A & 0 & 0 \\
C & 0 & -Z^{-1} S \\
\end{array}
\right)
\left(
\begin{array}{c}
\Delta x\\
\Delta y\\
-\Delta z\\
\end{array}
\right)
=
-\left(
\begin{array}{c}
r_x\\
r_y \\
r_z + Z^{-1} r_s
\end{array}
\right)
\]
This can be solved using a symmetric indefinite solver.

Using $C \Delta x + Z^{-1} S \Delta z = - (r_z + Z^{-1} r_s)$, we get
\[
\Delta z = -Z S^{-1} (C \Delta x + r_z + Z^{-1} r_s)
\]
which means that
\[
-C \Delta z = C Z S^{-1} C \Delta x + CZS^{-1} (r_z + Z^{-1} r_s)
\]
so we can reduce the system even more:
\[
\left(
\begin{array}{cccc}
H + C' ZS^{-1}C& A' \\
A & 0 \\
\end{array}
\right)
\left(
\begin{array}{c}
\Delta x\\
\Delta y\\
\end{array}
\right)
=
-\left(
\begin{array}{c}
r_x + C' Z S^{-1} (r_z + Z^{-1} r_s)\\
r_y \\
\end{array}
\right)
\]
If we had used a penalty $(1/2\mu) (Ax - b)' (Ax - b)$ with $y = (Ax-b)/\mu$, we would have had $-\mu I$ instead of the zero. In that case we could have used $A \Delta x - \mu \Delta y = - r_y$ to get
\[
\Delta y = (A \Delta x + r_y) / \mu
\]
which could be used to reduce the system to
\[
(H + C' Z S^{-1} C + A' A / \mu) \Delta x= - r_x  + C' S^{-1}(Z r_z + r_s)  + A' r_y / \mu

\]

\end{document}
